Add helper functions to organize pre and post conditions

managerOnlyUpdates - with changes.dfy
@@ -8,7 +8,14 @@ function arePublishersInBothLists (ads: map <Publisher, Ad>, publishers : seq<Pu
 	(forall p :: p in publishers ==> p in ads) && (forall p :: p in ads ==> p in publishers)
 }
 
+function valuesOfAds (myAds : map<Publisher, Ad>) : set<Ad>
+{
+	set p: Publisher | p in myAds :: myAds[p]
+}
+
 function isNoNullPublishers (ads: map <Publisher, Ad>, publishers : seq<Publisher>) : bool
+requires arePublishersInBothLists(ads, publishers)
+reads valuesOfAds(ads)
 {
 	forall p :: p in publishers ==> p != null && ads[p] != null && ads[p].banner != null
 }
@@ -32,6 +39,113 @@ function isPublisherInMap (publisher : Publisher, retAds: map <Publisher, Ad>) :
 {
 	publisher in retAds && retAds[publisher] != null
 }
+
+function checkStartPublishRoomInAvailableBanners(publisher : Publisher, price : int, publishers : seq<Publisher>, retPublishers: seq<Publisher>, ads : map <Publisher, Ad>, retAds: map <Publisher, Ad>, availableBanners : seq<Banner>, retBanners: seq<Banner>) : bool
+reads valuesOfAds(retAds)
+{
+	|availableBanners| > 0 ==> publisher in retPublishers && publisher in retAds && retAds[publisher] != null && retAds[publisher].price == price  && availableBanners[0] == retAds[publisher].banner && retBanners == availableBanners[1..] && availableBanners[0] !in retBanners
+}
+
+function checkStartPublishAllListsEmpty (publisher : Publisher, price : int, publishers : seq<Publisher>, retPublishers: seq<Publisher>, ads : map <Publisher, Ad>, retAds: map <Publisher, Ad>, availableBanners : seq<Banner>, retBanners: seq<Banner>) : bool
+{
+	(|availableBanners| == 0 && |publishers| == 0) ==> publishers == retPublishers && ads == retAds && availableBanners == retBanners && publisher !in publishers && publisher !in ads
+}
+
+function checkStartPublishBidAccepted (publisher : Publisher, price : int, publishers : seq<Publisher>, retPublishers: seq<Publisher>, ads : map <Publisher, Ad>, retAds: map <Publisher, Ad>, availableBanners : seq<Banner>, retBanners: seq<Banner>, globalMinPublisher: Publisher) : bool
+reads valuesOfAds(retAds)
+reads valuesOfAds(ads)
+requires forall p :: p in ads ==> ads[p] != null
+{
+	(|availableBanners| == 0 && |publishers| > 0 && !isPriceLessThanMinPrice(price, ads)) ==> (publisher in retPublishers && isPublisherInMap(publisher, retAds) && retAds[publisher].price == price && availableBanners == retBanners) && (globalMinPublisher !in retPublishers && globalMinPublisher !in retAds && globalMinPublisher in ads && retAds[publisher].banner == ads[globalMinPublisher].banner)
+}
+
+function isPriceLessThanMinPrice (price : int, ads: map <Publisher, Ad>) : bool
+reads valuesOfAds(ads)
+//requires forall p :: p in ads ==> ads[p] != null
+{
+	forall p :: p in ads && ads[p] != null ==> ads[p].price >= price
+}
+
+function checkStartPublishBidNotAccepted (publisher : Publisher, price : int, publishers : seq<Publisher>, retPublishers: seq<Publisher>, ads : map <Publisher, Ad>, retAds: map <Publisher, Ad>, availableBanners : seq<Banner>, retBanners: seq<Banner>) : bool
+reads valuesOfAds(ads)
+{
+	(|availableBanners| == 0 && |publishers| > 0 && isPriceLessThanMinPrice(price, ads)) ==> publishers == retPublishers && ads == retAds && availableBanners == retBanners && isPublisherOut(publisher, ads, publishers)
+}
+
+function isNoNull (availableBanners: seq<Banner>, publishers : seq<Publisher>, ads : map <Publisher, Ad>)  : bool
+reads valuesOfAds(ads)
+requires arePublishersInBothLists(ads, publishers)
+{
+	isNoNullPublishers(ads,publishers) && isNoNullAds(ads) && isNoNullAvailableBanners(availableBanners)
+}
+
+function adExists(adService : AdvertisingService, publisher: Publisher, ads: map <Publisher, Ad>, availableBanners: seq<Banner>) : bool
+reads valuesOfAds(ads)
+{
+	adService != null  && isPublisherInMap(publisher, ads) && ads[publisher].banner !in availableBanners 
+}
+
+function startPublishCorrectChanges (publisher: Publisher, availableBanners: seq<Banner>, publishers : seq<Publisher>, ads : map <Publisher, Ad>)  : bool
+reads valuesOfAds(ads)
+{
+	isPublisherOut(publisher, ads, publishers) && arePublishersInBothLists(ads, publishers) && isUniqueAvailableBanners(availableBanners) 
+}
+
+function findMinPublisherPreConditions(publishers : seq<Publisher>, ads : map <Publisher, Ad>) : bool 
+reads valuesOfAds(ads)
+{
+	|publishers| > 0 && forall p :: p in publishers ==> p != null && p in ads && ads[p] != null && ads[p].banner != null && arePublishersInBothLists(ads, publishers) && isNoNullAds(ads)
+}
+
+function findMinPublisherPostConditions(retPrice : int, retPublisher : Publisher, publishers : seq<Publisher>, ads : map <Publisher, Ad>) : bool 
+requires forall p :: p in ads ==> ads[p] != null
+reads valuesOfAds(ads)
+{
+	retPublisher in ads && retPublisher in publishers && retPublisher != null && ads[retPublisher] != null && ads[retPublisher].banner != null && ads[retPublisher].price == retPrice && forall p :: p in ads ==> ads[p].price >= retPrice
+}
+
+function startPublishPostConditions(publisher : Publisher, price : int, publishers : seq<Publisher>, retPublishers: seq<Publisher>, ads : map <Publisher, Ad>, retAds: map <Publisher, Ad>, availableBanners : seq<Banner>, retBanners: seq<Banner>, globalMinPublisher: Publisher) : bool
+reads valuesOfAds(retAds)
+reads valuesOfAds(ads)
+requires forall p :: p in ads ==> ads[p] != null
+{
+	checkStartPublishRoomInAvailableBanners(publisher, price, publishers, retPublishers, ads, retAds, availableBanners, retBanners)
+	&& checkStartPublishBidNotAccepted(publisher, price, publishers, retPublishers, ads, retAds, availableBanners, retBanners)
+	&& checkStartPublishBidAccepted(publisher, price, publishers, retPublishers, ads, retAds, availableBanners, retBanners, globalMinPublisher)
+	&& checkStartPublishAllListsEmpty(publisher, price, publishers, retPublishers, ads, retAds, availableBanners, retBanners)
+}
+
+function removePublisherInvPublisherOut(index: int, publishers: seq<Publisher>, newPublishers: seq<Publisher>, publisher: Publisher) : bool
+{
+	0 <= index <= |publishers| && publisher !in newPublishers
+}
+
+function removePublisherInvRestIn(index: int, publishers: seq<Publisher>, newPublishers: seq<Publisher>, publisher: Publisher) : bool
+requires index <= |publishers|
+{
+	forall i :: 0 <= i < index && publishers[i] != publisher ==> publishers[i] in newPublishers
+}
+
+
+function findMinPublisherInvDataStructuresOk(minPrice: int, ads : map <Publisher, Ad>, index: int, publishers: seq<Publisher>, minPublisher: Publisher) : bool
+reads valuesOfAds(ads)
+{
+	forall p :: p in publishers ==> p in ads && minPublisher in ads && ads[minPublisher] != null && ads[minPublisher].price == minPrice && minPublisher in publishers
+}
+
+function findMinPublisherInvMinPriceCorrect(minPrice: int, ads : map <Publisher, Ad>, index: int, publishers: seq<Publisher>, minPublisher: Publisher) : bool
+requires isNoNullAds(ads)
+requires arePublishersInBothLists(ads, publishers)
+reads valuesOfAds(ads)
+{
+	0 <= index <= |publishers| && minPublisher in ads && forall i :: 0 <= i < index ==> minPrice <= ads[publishers[i]].price && isNoNullAds(ads)
+}
+
+
+
+
+
+
 
 
 
@@ -79,9 +193,7 @@ class AdvertisingManager {
     
     method stopPublish (publisher: Publisher) 
     modifies this
-    requires adService != null 
-    requires isPublisherInMap(publisher, ads)
-    requires ads[publisher].banner !in availableBanners 
+	requires adExists(adService, publisher, ads, availableBanners)
     //requires banner !in availableBanners    
     //ensures publisher !in publishers
     //ensures publisher !in ads
@@ -95,19 +207,13 @@ class AdvertisingManager {
     method startPublish (publisher : Publisher, price : int) 
     modifies this
     modifies adService
-    requires adService != null  
-    requires isPublisherOut(publisher, ads, publishers)
 	requires arePublishersInBothLists(ads, publishers)
-    requires isNoNullPublishers(ads, publishers)
-	requires isNoNullAds(ads)
-    requires isNoNullAvailableBanners(availableBanners)
-    requires isUniqueAvailableBanners(availableBanners)
+	requires isNoNull (availableBanners, publishers, ads) &&  adService != null
+	requires startPublishCorrectChanges(publisher, availableBanners, publishers, ads)
     {
         publishers, ads, availableBanners := adService.startPublish(publisher, price, publishers, ads, availableBanners);
     }        
 }
-
-
 
 class AdvertisingService 
 {
@@ -145,8 +251,8 @@ class AdvertisingService
         var newPublishers : seq<Publisher> := [];
         while (index < |publishers|)
         decreases |publishers| - index // not needed - but it seems more complicated :)
-        invariant 0 <= index <= |publishers| && publisher !in newPublishers
-        invariant forall i :: 0 <= i < index && publishers[i] != publisher ==> publishers[i] in newPublishers
+        invariant removePublisherInvPublisherOut(index, publishers, newPublishers, publisher)
+        invariant removePublisherInvRestIn(index, publishers, newPublishers, publisher)
         {
             if (publishers[index] != publisher)
             {
@@ -190,14 +296,9 @@ class AdvertisingService
     
     // WE CAN NOW CHANGE THIS METHOD TO USE THE NEW FUNCTIONS - BUT IT MAY CHANGE THE CONDITIONS :( 
     method findMinPublisher(publishers : seq<Publisher>, ads : map <Publisher, Ad>) returns (retPublisher : Publisher, retPrice : int)
-    requires |publishers| > 0
-    requires forall p :: p in publishers ==> p != null && p in ads && ads[p] != null && ads[p].banner != null
-    requires arePublishersInBothLists(ads, publishers)
-	requires isNoNullAds(ads)
-    ensures retPublisher in ads && retPublisher in publishers
-    ensures retPublisher != null && ads[retPublisher] != null && ads[retPublisher].banner != null
-    ensures ads[retPublisher].price == retPrice
-  	ensures forall p :: p in ads ==> ads[p].price >= retPrice // also true forall :: p in publishers... 
+	requires findMinPublisherPreConditions(publishers, ads)
+	requires forall p :: p in ads ==> ads[p] != null
+	ensures findMinPublisherPostConditions(retPrice, retPublisher, publishers, ads)
     {
       var minPublisher := publishers[0];
       var minPrice := ads[minPublisher].price;
@@ -205,8 +306,8 @@ class AdvertisingService
       var index := 1;
       while (index < |publishers|)
       decreases |publishers| - index
-      invariant  forall p :: p in publishers ==> p in ads && minPublisher in ads && ads[minPublisher] != null && ads[minPublisher].price == minPrice && minPublisher in publishers 
-      invariant 0 <= index <= |publishers| && minPublisher in ads && forall i :: 0 <= i < index ==> minPrice <= ads[publishers[i]].price && isNoNullAds(ads)
+	  invariant findMinPublisherInvDataStructuresOk(minPrice, ads, index, publishers, minPublisher)
+	  invariant findMinPublisherInvMinPriceCorrect(minPrice, ads, index, publishers, minPublisher)
 	  // checkInvariantFindMinPublisher(index, publishers, ads,minPublisher, minPrice);
 	  {
         var curPrice := ads[publishers[index]].price;
@@ -220,17 +321,6 @@ class AdvertisingService
       return minPublisher, minPrice;
     }    
     
-	function isPriceLessThanMinPrice (price : int, ads: map <Publisher, Ad>) : bool
-    reads valuesOfAds(ads)
-    //requires forall p :: p in ads ==> ads[p] != null
-    {
-      forall p :: p in ads && ads[p] != null ==> ads[p].price >= price
-    }
-    
-    function valuesOfAds (myAds : map<Publisher, Ad>) : set<Ad>
-    {
-      set p: Publisher | p in myAds :: myAds[p]
-    }
 
 /*
     // need to add ensures...     
@@ -253,32 +343,17 @@ class AdvertisingService
     }
     */
     
-	//function checkStartPublishAllListsEmpty (publisher : Publisher, price : int, publishers : seq<Publisher>, retPublishers: seq<Publisher>, ads : map <Publisher, Ad>, retAds: map <Publisher, Ad>, availableBanners : seq<Banner>, retBanners: seq<Banner>) : bool
-    //{
-      //(|availableBanners| == 0 && |publishers| == 0) ==> publishers == retPublishers && ads == retAds && availableBanners == retBanners && publisher !in publishers && publisher !in ads
-    //}
 
-	//function checkStartPublishRoomInAvailableBanners(publisher : Publisher, price : int, publishers : seq<Publisher>, retPublishers: seq<Publisher>, ads : map <Publisher, Ad>, retAds: map <Publisher, Ad>, availableBanners : seq<Banner>, retBanners: seq<Banner>) : bool
-	//{
-		//|availableBanners| > 0 ==> publisher in retPublishers && publisher in retAds && retAds[publisher] != null && retAds[publisher].price == price  && availableBanners[0] == retAds[publisher].banner && retBanners == availableBanners[1..] && availableBanners[0] !in retBanners
-	//}
+
+
+
 
     method startPublish(publisher : Publisher, price : int, publishers : seq<Publisher>, ads : map <Publisher, Ad>, availableBanners : seq<Banner>) returns (retPublishers : seq<Publisher>, retAds : map <Publisher, Ad>, retBanners : seq<Banner>)
     modifies this
-    requires isPublisherOut(publisher, ads, publishers);
-    requires arePublishersInBothLists(ads, publishers)
-    requires isNoNullPublishers(ads,publishers)
-	requires isNoNullAds(ads)
-    requires isNoNullAvailableBanners(availableBanners)
-    requires isUniqueAvailableBanners(availableBanners)  
 	
-	ensures |availableBanners| > 0 ==> publisher in retPublishers && isPublisherInMap(publisher, retAds) && retAds[publisher].price == price  && availableBanners[0] == retAds[publisher].banner && retBanners == availableBanners[1..] && availableBanners[0] !in retBanners
-    //ensures checkStartPublishRoomInAvailableBanners(publisher, price, publishers, retPublishers, ads, retAds, availableBanners, retBanners);
-	ensures (|availableBanners| == 0 && |publishers| > 0 && isPriceLessThanMinPrice(price, ads)) ==> publishers == retPublishers && ads == retAds && availableBanners == retBanners && isPublisherOut(publisher, ads, publishers)
-	ensures (|availableBanners| == 0 && |publishers| > 0 && !isPriceLessThanMinPrice(price, ads)) ==> publisher in retPublishers && isPublisherInMap(publisher, retAds) && retAds[publisher].price == price && availableBanners == retBanners 
-    ensures |availableBanners| == 0 && |publishers| > 0 && !isPriceLessThanMinPrice(price, ads) ==> globalMinPublisher !in retPublishers && globalMinPublisher !in retAds && globalMinPublisher in ads && retAds[publisher].banner == ads[globalMinPublisher].banner 
-	ensures (|availableBanners| == 0 && |publishers| == 0) ==> publishers == retPublishers && ads == retAds && availableBanners == retBanners && isPublisherOut(publisher, ads, publishers)
-	//ensures  checkStartPublishAllListsEmpty(publisher, price, publishers, retPublishers, ads, retAds, availableBanners, retBanners);
+	requires startPublishCorrectChanges(publisher, availableBanners, publishers, ads)
+	requires isNoNull (availableBanners, publishers, ads) 
+	ensures startPublishPostConditions(publisher, price, publishers, retPublishers, ads, retAds, availableBanners, retBanners, globalMinPublisher);
 
 	{
       var newPublishers : seq<Publisher> := publishers;
